theories/typechecker/typechecker.v
@@ -12,10 +12,11 @@ Definition type_checker_res := sum ok type_error.
 Definition ok_term : type_checker_res := inl ().
 Definition INR (s:string) : type_checker_res := inr s.
 
+Hint Unfold ok_term : core.
 
 
 (* No matter how type_checker_res changes, this MUST stay the same *)
-Definition check_ok In (func: In -> type_checker_res) (i: In) : bool :=
+Definition check_ok {In} (func: In -> type_checker_res) (i: In) : bool :=
   match (func i) with
   | inl a => true
   | inr a => false
@@ -29,8 +30,8 @@ Definition check_ok_output (res: type_checker_res) : bool :=
 
 (* This is only true if ok is kept at unit. Unfortunately most of the proofs
  rely on this. *)
-Lemma check_ok_true_to_prop In (func: In -> type_checker_res) (i:In) :
-  check_ok In func i = true -> func i = ok_term.
+Lemma check_ok_true_to_prop {In} (func: In -> type_checker_res) (i:In) :
+  check_ok func i = true -> func i = ok_term.
 Proof.
   intros. unfold ok_term.
   destruct (func i) eqn:H'.
@@ -68,15 +69,27 @@ Proof.
 Qed.
 
 (* Converting between _ = ok_term to check_ok = true *)
-Lemma equal_okterm_to_checkok In (func: In -> type_checker_res) (Pbool : In -> Prop) :
+Lemma equal_okterm_to_checkok {In} (func: In -> type_checker_res) (Pbool : In -> Prop) :
   forall i:In,
     ((func i = ok_term -> Pbool i) ->
-     (check_ok In func i = true -> Pbool i)).
+     (check_ok func i = true -> Pbool i)).
 Proof.
   intros. apply H.
   by apply check_ok_true_to_prop.
 Qed.
 
+(* A few tactics *)
+Ltac solve_Forall_foldr HForall Hfoldr checker proper :=
+  apply (Forall_impl _ (λ x, check_ok checker x = true -> proper x)) in HForall;
+  [ eapply Forall_foldr_bool_to_prop; [apply HForall | apply Hfoldr] |
+    ( (by apply equal_okterm_to_checkok) ||
+      (intros; eapply equal_okterm_to_checkok; [ | eassumption ]; auto)) ].
+
+Ltac destruct_on_if_equal resname :=
+  match goal with
+    | H:((if ?key then _ else _)=_) |- _ => destruct key eqn:resname
+  end
+.
 
 
 
@@ -112,10 +125,10 @@ Fixpoint rep_ok_checker (k:kind_ctx) (rep:representation) : type_checker_res :=
   | AtomR ι => ok_term
   | VarR r => if r <? k.(kc_rep_vars) then ok_term else INR "rep_ok error"
   | ProdR ρs =>
-      if (foldr (λ i:representation, andb (check_ok representation (rep_ok_checker k) i)) true ρs)
+      if (foldr (λ i:representation, andb (check_ok (rep_ok_checker k) i)) true ρs)
            then ok_term else INR "rep_ok error"
   | SumR ρs =>
-       if (foldr (λ i:representation, andb (check_ok representation (rep_ok_checker k) i)) true ρs)
+       if (foldr (λ i:representation, andb (check_ok (rep_ok_checker k) i)) true ρs)
            then ok_term else INR "rep_ok error"
  end.
 
@@ -123,28 +136,13 @@ Lemma rep_ok_checker_correct (k:kind_ctx) (rep:representation) :
   (rep_ok_checker k rep = ok_term) -> rep_ok k rep.
 Proof.
   intros.
-  induction rep using rep_ind.
+  induction rep using rep_ind; simpl in H.
   - apply OKVarR.
-    simpl in H.
-    destruct (idx <? kc_rep_vars k) eqn:H'.
-    + apply Nat.ltb_lt in H'. auto.
-    + inversion H.
+    destruct_on_if_equal H'; [apply Nat.ltb_lt in H'; auto | inversion H].
   - apply OKSumR.
-    simpl in H.
-    destruct (foldr (λ i:representation, andb (check_ok representation (rep_ok_checker k) i)) true ρs) eqn:H'.
-    + clear H.
-      apply (Forall_impl _ (λ x, check_ok representation (rep_ok_checker k) x = true -> rep_ok k x)) in H0.
-      * eapply Forall_foldr_bool_to_prop; [apply H0 | apply H'].
-      * apply equal_okterm_to_checkok.
-    + inversion H.
+    destruct_on_if_equal Hfoldr; [solve_Forall_foldr H0 Hfoldr (rep_ok_checker k) (rep_ok k) | inversion H].
   - apply OKProdR.
-    simpl in H.
-    destruct (foldr (λ i:representation, andb (check_ok representation (rep_ok_checker k) i)) true ρs) eqn:H'.
-    + clear H.
-      apply (Forall_impl _ (λ x, check_ok representation (rep_ok_checker k) x = true -> rep_ok k x)) in H0.
-      * eapply Forall_foldr_bool_to_prop; [apply H0 | apply H'].
-      * apply equal_okterm_to_checkok.
-    + inversion H.
+    destruct_on_if_equal Hfoldr; [solve_Forall_foldr H0 Hfoldr (rep_ok_checker k) (rep_ok k) | inversion H].
   - apply OKAtomR.
 Qed.
 
@@ -162,10 +160,10 @@ Fixpoint size_ok_checker (k:kind_ctx) (s:size) : type_checker_res :=
                           better for future changeability. I'll do just ret later*)
               end
   | SumS σs =>
-      if (foldr (λ i:size, andb (check_ok size (size_ok_checker k) i)) true σs)
+      if (foldr (λ i:size, andb (check_ok (size_ok_checker k) i)) true σs)
            then ok_term else INR "size_ok error"
   | ProdS σs =>
-      if (foldr (λ i:size, andb (check_ok size (size_ok_checker k) i)) true σs)
+      if (foldr (λ i:size, andb (check_ok (size_ok_checker k) i)) true σs)
            then ok_term else INR "size_ok error"
   end.
 
@@ -173,28 +171,13 @@ Lemma size_ok_checker_correct (k:kind_ctx) (s:size) :
   (size_ok_checker k s = ok_term) -> size_ok k s.
 Proof.
   intros.
-  induction s using size_ind.
+  induction s using size_ind; simpl in H.
   - apply OKVarS.
-    simpl in H.
-    destruct (idx <? kc_size_vars k) eqn:H'.
-    + apply Nat.ltb_lt in H'. auto.
-    + inversion H.
+    destruct_on_if_equal H'; [apply Nat.ltb_lt in H'; auto | inversion H].
   - apply OKSumS.
-    simpl in H.
-    destruct (foldr (λ i:size, andb (check_ok size (size_ok_checker k) i)) true σs) eqn:H'.
-    + clear H.
-      apply (Forall_impl _ (λ x, check_ok size (size_ok_checker k) x = true -> size_ok k x)) in H0.
-      * eapply Forall_foldr_bool_to_prop; [apply H0 | apply H'].
-      * apply equal_okterm_to_checkok.
-    + inversion H.
+    destruct_on_if_equal Hfoldr; [solve_Forall_foldr H0 Hfoldr (size_ok_checker k) (size_ok k) | inversion H].
   - apply OKProdS.
-    simpl in H.
-    destruct (foldr (λ i:size, andb (check_ok size (size_ok_checker k) i)) true σs) eqn:H'.
-    + clear H.
-      apply (Forall_impl _ (λ x, check_ok size (size_ok_checker k) x = true -> size_ok k x)) in H0.
-      * eapply Forall_foldr_bool_to_prop; [apply H0 | apply H'].
-      * apply equal_okterm_to_checkok.
-    + inversion H.
+    destruct_on_if_equal Hfoldr; [solve_Forall_foldr H0 Hfoldr (size_ok_checker k) (size_ok k) | inversion H].
   - apply OKRepS.
     simpl in H.
     destruct (rep_ok_checker k ρ) eqn:H'.
@@ -224,3 +207,165 @@ Proof.
   - apply OKMEMTYPE.
     apply size_ok_checker_correct; auto.
 Qed.
+
+
+(* type_ok *)
+Fixpoint type_ok_checker (F:function_ctx) (t:type) : type_checker_res :=
+  match t with
+  | VarT t => match (F.(fc_type_vars) !! t) with
+              | Some κ => kind_ok_checker (F.(fc_kind_ctx)) κ
+              | None => INR "type ok error"
+              end
+  | I31T κ => kind_ok_checker (F.(fc_kind_ctx)) κ
+  | NumT κ ν => kind_ok_checker (F.(fc_kind_ctx)) κ
+  | SumT κ τs | VariantT κ τs | ProdT κ τs | StructT κ τs
+    => match (kind_ok_checker (F.(fc_kind_ctx)) κ) with
+       | inl ()  =>
+           if (foldr (λ t:type, andb (check_ok (type_ok_checker F) t)) true τs)
+           then ok_term else INR "type ok error"
+       | err => err
+       end
+  | RefT κ μ τ =>
+      match (kind_ok_checker (F.(fc_kind_ctx)) κ) with
+      | inl () =>
+          match (mem_ok_checker (F.(fc_kind_ctx)) μ) with
+          | inl () => type_ok_checker F τ
+          | err => err
+          end
+      | err => err
+      end
+  | CodeRefT κ ft =>
+      match (kind_ok_checker (F.(fc_kind_ctx)) κ) with
+      | inl () => function_type_ok_checker F ft
+      | err => err
+      end
+  | SerT κ τ =>
+      match (kind_ok_checker (F.(fc_kind_ctx)) κ) with
+      | inl () => type_ok_checker F τ
+      | err => err
+      end
+  | PlugT κ ρ =>
+      match (kind_ok_checker (F.(fc_kind_ctx)) κ) with
+      | inl () => rep_ok_checker (F.(fc_kind_ctx)) ρ
+      | err => err
+      end
+  | SpanT κ σ =>
+      match (kind_ok_checker (F.(fc_kind_ctx)) κ) with
+      | inl () => size_ok_checker (F.(fc_kind_ctx)) σ
+      | err => err
+      end
+  | RecT κ τ =>
+      match (kind_ok_checker (F.(fc_kind_ctx)) κ) with
+      | inl () => type_ok_checker (F <| fc_type_vars ::= cons κ |>) τ
+      | err => err
+      end
+  | ExistsMemT κ τ =>
+      match (kind_ok_checker (F.(fc_kind_ctx)) κ) with
+      | inl () => type_ok_checker (F <| fc_kind_ctx ::= set kc_mem_vars S |>) τ
+      | err => err
+      end
+  | ExistsRepT κ τ =>
+      match (kind_ok_checker (F.(fc_kind_ctx)) κ) with
+      | inl () => type_ok_checker (F <| fc_kind_ctx ::= set kc_rep_vars S |>) τ
+      | err => err
+      end
+  | ExistsSizeT κ τ =>
+      match (kind_ok_checker (F.(fc_kind_ctx)) κ) with
+      | inl () => type_ok_checker (F <| fc_kind_ctx ::= set kc_size_vars S |>) τ
+      | err => err
+      end
+  | ExistsTypeT κ1 κ2 τ =>
+     match (kind_ok_checker (F.(fc_kind_ctx)) κ1) with
+     | inl () =>
+         match (kind_ok_checker (F.(fc_kind_ctx)) κ2) with
+         | inl () => type_ok_checker (F <| fc_type_vars ::= cons κ2 |>) τ
+         | err => err
+         end
+     | err => err
+     end
+  end
+    with function_type_ok_checker (F: function_ctx) (ft:function_type) : type_checker_res :=
+      match ft with
+      | MonoFunT τs1 τs2 =>
+           if (foldr (λ t:type, andb (check_ok (type_ok_checker F) t)) true τs1)
+           then
+              if (foldr (λ t:type, andb (check_ok (type_ok_checker F) t)) true τs2)
+              then ok_term
+              else INR "function type ok error"
+           else INR "function type ok error"
+      | ForallMemT ϕ => function_type_ok_checker (F <| fc_kind_ctx ::= set kc_mem_vars S |>) ϕ
+      | ForallRepT ϕ => function_type_ok_checker (F <| fc_kind_ctx ::= set kc_rep_vars S |>) ϕ
+      | ForallSizeT ϕ => function_type_ok_checker (F <| fc_kind_ctx ::= set kc_size_vars S |>) ϕ
+      | ForallTypeT κ ϕ =>
+          match (kind_ok_checker (F.(fc_kind_ctx)) κ) with
+          | inl () => function_type_ok_checker (F <| fc_type_vars ::= cons κ |>) ϕ
+          | err => err
+          end
+      end.
+
+Ltac destruct_match_kind_ok F κ o Hres HMatchKind :=
+  destruct (kind_ok_checker (fc_kind_ctx F) κ) eqn:Hres; [ | inversion HMatchKind ];
+  unfold ok in o; assert (o = tt) by (by destruct o); subst.
+
+Ltac destruct_on_match_equal resname :=
+  match goal with
+  | H: ((match ?key with |_=>_ end) = _) |- _ => destruct key eqn:resname
+  end.
+
+Ltac stupid_unit o :=
+  unfold ok in o; assert (HO: o = tt) by (by destruct o); subst.
+
+Ltac destruct_match_unit Hmatch resname o :=
+  destruct_on_match_equal resname; [stupid_unit o | inversion Hmatch].
+
+Ltac my_auto :=
+  match goal with
+  | H: ((match ?key with |_=>_ end) = _) |- _ => destruct key eqn:?HMatch; [ | inversion H ]
+  | H:((if ?key then _ else _)=_) |- _ => destruct key eqn:?HMatch; [ | inversion H ]
+  | o:ok |- _ => stupid_unit o
+  | H: (kind_ok_checker _ _ = inl ()) |- _ => apply kind_ok_checker_correct in H; auto
+  | H: (kind_ok_checker _ _ = ok_term) |- _ => apply kind_ok_checker_correct in H; auto
+  | H: (mem_ok_checker _ _ = inl ()) |- _ => apply mem_ok_checker_correct in H; auto
+  | H: (mem_ok_checker _ _ = ok_term) |- _ => apply mem_ok_checker_correct in H; auto
+  | H: (rep_ok_checker _ _ = inl ()) |- _ => apply rep_ok_checker_correct in H; auto
+  | H: (rep_ok_checker _ _ = ok_term) |- _ => apply rep_ok_checker_correct in H; auto
+  | H: (size_ok_checker _ _ = inl ()) |- _ => apply size_ok_checker_correct in H; auto
+  | H: (size_ok_checker _ _ = ok_term) |- _ => apply size_ok_checker_correct in H; auto
+end.
+
+Ltac find_Forall_foldr checker prop :=
+  match goal with
+  | HForall: ((Forall _ _)), Hfoldr: (foldr _ _ _ = _) |- _ =>
+      solve_Forall_foldr HForall Hfoldr checker prop
+  end.
+
+Lemma type_ok_checker_correct :
+  (forall t F, (type_ok_checker F t = ok_term) -> type_ok F t) /\
+  (forall ft F, function_type_ok_checker F ft = ok_term -> function_type_ok F ft).
+Proof.
+
+  Ltac auto_local F := repeat my_auto; try find_Forall_foldr (type_ok_checker F) (type_ok F); auto.
+
+  apply type_and_function_ind.
+  1-17, 19-22: intros; simpl in H; try simpl in H0;
+    try(constructor; auto_local F). (* this solves a LOT of cases *)
+  - (* The var case requires econstructor, which I didn't want to do in general *)
+    auto_local F; econstructor; eassumption.
+  - (* The monofun case has to be done manually bc my find_Forall_foldr isn't that smart *)
+    intros; simpl in H. simpl in H1.
+    repeat my_auto.
+    constructor.
+    + solve_Forall_foldr H HMatch (type_ok_checker F) (type_ok F); auto.
+    + solve_Forall_foldr H0 HMatch0 (type_ok_checker F) (type_ok F); auto.
+
+Qed.
+
+
+(* Have to define an equality operator on representation and dropability *)
+Fixpoint subkind_of_checker (κ1:kind) (κ2:kind) : type_checker_res :=
+  match κ1, κ2 with
+  | (VALTYPE ρ1 ImCopy δ1), (VALTYPE ρ2 ExCopy δ2) =>
+      (* this true here is fake *)
+      if true then ok_term else INR "not subkind"
+  | _, _ => INR "no"
+  end.
